Phi_Semantics/PhiSem_Variable2.thy
@@ -1,0 +1,551 @@
+chapter \<open>Typed Variable\<close>
+
+text \<open>This is a generic formalization variables supporting either typed variables or non-typed.
+If the formalization is untyped, variables in the formalization can be assigned by values of
+any type.
+You can set the flag \<phi>variable_is_typed to indicate whether the formalization of variables is typed.\<close>
+
+theory PhiSem_Variable2
+  imports Phi_System.Resource_Template
+  abbrevs "<var>" = "\<v>\<a>\<r>"
+begin
+
+section \<open>Semantics\<close>
+
+subsection \<open>Models\<close>
+
+subsubsection \<open>Resource\<close>
+
+declare [[typedef_overloaded]]
+datatype varname = varname nat \<comment> \<open>nonce\<close> (type: \<open>TY option\<close>) \<comment> \<open>None denotes no type restriction.\<close>
+hide_const (open) type
+declare [[typedef_overloaded = false]]
+
+setup \<open>Sign.mandatory_path "RES"\<close>
+
+type_synonym Var = \<open>varname \<rightharpoonup> VAL option nosep\<close>
+  \<comment> \<open>NONE: declared but not initialized.\<close>
+
+setup \<open>Sign.parent_path\<close>
+
+lemma infinite_varname:
+  \<open>infinite {k. varname.type k = TY}\<close>
+  using inj_on_finite[where A = \<open>UNIV::nat set\<close> and B = \<open>{k. varname.type k = TY}\<close>
+        and f = \<open>\<lambda>n. varname n TY\<close>]
+  using inj_def by fastforce
+
+resource_space \<phi>var =
+  Var  :: \<open>{vars::RES.Var. finite (dom vars)}\<close> (partial_map_resource) ..
+
+hide_fact RES.\<phi>var_res_ax RES.\<phi>var_res_axioms RES.\<phi>var_res_fields_axioms
+
+
+subsubsection \<open>Fiction\<close>
+
+fiction_space \<phi>var =
+  Var :: \<open>RES.Var.basic_fiction o\<^sub>\<I> \<F>_pointwise \<F>_it\<close> (pointwise_fiction_for_partial_mapping_resource RES.Var) ..
+
+hide_fact FIC.\<phi>var_fic_ax FIC.\<phi>var_fic_axioms
+
+
+
+section \<open>\<phi>-Types\<close>
+
+subsection \<open>Variable\<close>
+
+abbreviation Var :: \<open>varname \<Rightarrow> (VAL option,'a) \<phi> \<Rightarrow> (fiction,'a) \<phi>\<close>
+  where \<open>Var vname T \<equiv> (FIC.Var.\<phi> (vname \<^bold>\<rightarrow> \<black_circle> (Nosep T)))\<close>
+
+abbreviation Inited_Var :: \<open>varname \<Rightarrow> (VAL,'a) \<phi> \<Rightarrow> (fiction,'a) \<phi>\<close>
+  where \<open>Inited_Var vname T \<equiv> Var vname (\<black_circle> T)\<close>
+
+abbreviation Uninited_Var :: \<open>varname \<Rightarrow> assn\<close> ("\<u>\<n>\<i>\<n>\<i>\<t>\<e>\<d> \<v>\<a>\<r>[_]" [22] 21)
+  where \<open>Uninited_Var vname \<equiv> () \<Ztypecolon> Var vname \<circle>\<close>
+
+subsubsection \<open>Syntax\<close>
+
+syntax Inited_Var_ :: \<open>logic \<Rightarrow> logic\<close> ("\<v>\<a>\<r>[_]")
+
+ML_file "library/variable_pre.ML"
+
+parse_translation \<open>let
+
+fun get_bound ctxt (Const (\<^syntax_const>\<open>_constrain\<close>, _) $ X $ _) = get_bound ctxt X
+  | get_bound ctxt (Free (N, _)) = Option.map (K N) (Generic_Variable_Access.lookup_bindings ctxt N)
+  | get_bound _ _ = NONE
+
+in [
+  (\<^syntax_const>\<open>Inited_Var_\<close>, (fn ctxt => fn [v] =>
+    Const (\<^const_abbrev>\<open>Inited_Var\<close>, dummyT)
+        $ (if Generic_Variable_Access.is_under_value_context ctxt
+           then (case get_bound ctxt v
+                   of SOME N => Const (\<^const_name>\<open>\<phi>identifier\<close>, dummyT) $ Abs (N, dummyT, Term.dummy)
+                    | NONE => v)
+           else v)))
+] end\<close>
+
+print_translation \<open>let
+
+fun recovery ctxt (Const (\<^syntax_const>\<open>_free\<close>, _) $ X) = recovery ctxt X
+  | recovery ctxt (Free (N, TY)) =
+     (case Phi_Variable.external_name_of ctxt N
+        of SOME N' => SOME (Free (N', TY))
+         | _       => NONE)
+  | recovery ctxt (Var ((N,idx), TY)) =
+     (case Phi_Variable.external_name_of ctxt N
+        of SOME N' => SOME (Var ((N',idx), TY))
+         | _       => NONE)
+  | recovery _ _ = NONE
+
+fun recovery' ctxt X = case recovery ctxt X of SOME Y => Y | _ => X
+
+in [(\<^const_syntax>\<open>Inited_Var\<close>, (fn ctxt => fn [a,b] =>
+      Const(\<^syntax_const>\<open>Inited_Var_\<close>, dummyT) $ recovery' ctxt a $ b))]
+end
+\<close>
+
+lemma [\<phi>reason 2000 for
+  \<open>Synthesis_Parse (?var::varname) (?Y::?'ret \<Rightarrow> assn)\<close>
+]:
+  \<open>Synthesis_Parse var (\<lambda>_. x \<Ztypecolon> Var var T :: assn)\<close>
+  unfolding Synthesis_Parse_def ..
+
+lemma [\<phi>reason 2000 for
+  \<open>Synthesis_Parse (Var ?var) (?Y::?'ret \<Rightarrow> assn)\<close>
+]:
+  \<open>Synthesis_Parse (Var var) (\<lambda>_. x \<Ztypecolon> Var var T :: assn)\<close>
+  unfolding Synthesis_Parse_def ..
+
+lemma [\<phi>reason 2000 for
+  \<open>Synthesis_Parse (Inited_Var ?var) (?Y::?'ret \<Rightarrow> assn)\<close>
+]:
+  \<open>Synthesis_Parse (Inited_Var var) (\<lambda>_. x \<Ztypecolon> Inited_Var var T :: assn)\<close>
+  unfolding Synthesis_Parse_def ..
+
+lemma [\<phi>reason 2000 for
+  \<open>Synthesis_Parse (Uninited_Var ?var) (?Y::?'ret \<Rightarrow> assn)\<close>
+]:
+  \<open>Synthesis_Parse (Uninited_Var var) (\<lambda>_. Uninited_Var var :: assn)\<close>
+  unfolding Synthesis_Parse_def ..
+
+
+
+subsubsection \<open>Properties\<close>
+
+lemma Var_inhabited[\<phi>inhabitance_rule,elim!]:
+  \<open>Inhabited (x \<Ztypecolon> Var vname T) \<Longrightarrow> (Inhabited (x \<Ztypecolon> T) \<Longrightarrow> C) \<Longrightarrow> C\<close>
+  unfolding Inhabited_def by (simp add: \<phi>expns)
+
+lemma Var_transformation:
+  \<open> x \<Ztypecolon> T \<i>\<m>\<p>\<l>\<i>\<e>\<s> x' \<Ztypecolon> T' \<a>\<n>\<d> P
+\<Longrightarrow> x \<Ztypecolon> Var v T \<i>\<m>\<p>\<l>\<i>\<e>\<s> x' \<Ztypecolon> Var v T' \<a>\<n>\<d> P\<close>
+  unfolding Imply_def by (simp add: \<phi>expns, blast)
+
+lemma Var_cast_\<phi>app[\<phi>overload cast]:
+  \<open> \<^bold>a\<^bold>r\<^bold>g\<^bold>u\<^bold>m\<^bold>e\<^bold>n\<^bold>t x \<Ztypecolon> T \<i>\<m>\<p>\<l>\<i>\<e>\<s> x' \<Ztypecolon> T' \<a>\<n>\<d> P
+\<Longrightarrow> x \<Ztypecolon> \<v>\<a>\<r>[v] T \<i>\<m>\<p>\<l>\<i>\<e>\<s> x' \<Ztypecolon> \<v>\<a>\<r>[v] T' \<a>\<n>\<d> P\<close>
+  unfolding Argument_def
+  unfolding Imply_def View_Shift_def
+  by (clarsimp simp add: \<phi>expns, metis)
+
+lemma Raw_Var_identity_eq:
+  \<open>(raw \<Ztypecolon> Var v Identity) = (1(v \<mapsto> nosep raw) \<Ztypecolon> FIC.Var.\<phi> Identity)\<close>
+  unfolding set_eq_iff by (simp add: \<phi>expns)
+
+lemma UnInited_Var_identity_eq:
+  \<open>(\<u>\<n>\<i>\<n>\<i>\<t>\<e>\<d> \<v>\<a>\<r>[v]) = (nosep None \<Ztypecolon> FIC.Var.\<phi> (v \<^bold>\<rightarrow> \<black_circle> Identity))\<close>
+  unfolding set_eq_iff by (simp add: \<phi>expns)
+
+lemma Inited_Var_identity_eq:
+  \<open>(raw \<Ztypecolon> \<v>\<a>\<r>[v] Identity) = (1(v \<mapsto> nosep (Some raw)) \<Ztypecolon> FIC.Var.\<phi> Identity)\<close>
+  unfolding set_eq_iff by (simp add: \<phi>expns)
+
+(* lemma Var_ExTyp[simp]:
+  \<open>(x \<Ztypecolon> Var vname (ExTyp T)) = (\<exists>*a. x a \<Ztypecolon> Var vname (T a))\<close>
+  unfolding set_eq_iff by (simp add: \<phi>expns)
+
+lemma Var_SubjTyp[simp]:
+  \<open>(x \<Ztypecolon> Var vname (T \<phi>\<s>\<u>\<b>\<j> P)) = (x \<Ztypecolon> Var vname T \<s>\<u>\<b>\<j> P)\<close>
+  unfolding set_eq_iff by (simp add: \<phi>expns) *)
+
+(*lemma [\<phi>reason 1200 for \<open>EqualAddress (?xa \<Ztypecolon> Var ?va ?Ta) (?xb \<Ztypecolon> Var ?vb ?Tb)\<close>]:
+  \<open>EqualAddress (xa \<Ztypecolon> Var var Ta) (xb \<Ztypecolon> Var var Tb)\<close>
+  unfolding EqualAddress_def .. *)
+
+
+subsubsection \<open>Rules\<close>
+
+lemma [\<phi>reason 1305 for \<open>_\<heavy_comma> _ \<Ztypecolon> Var _ _ \<i>\<m>\<p>\<l>\<i>\<e>\<s> _\<heavy_comma> \<blangle> _ \<Ztypecolon> Var _ _ \<brangle> \<a>\<n>\<d> _\<close>]:
+  " R\<heavy_comma> x \<Ztypecolon> Var var T \<i>\<m>\<p>\<l>\<i>\<e>\<s> R\<heavy_comma> \<blangle> x \<Ztypecolon> Var var T \<brangle> "
+  unfolding Action_Tag_def FOCUS_TAG_def
+  using implies_refl by blast
+
+lemma [\<phi>reason 1300 for \<open>_\<heavy_comma> _ \<Ztypecolon> Var _ _ \<i>\<m>\<p>\<l>\<i>\<e>\<s> _\<heavy_comma> \<blangle> _ \<Ztypecolon> Var _ _ \<brangle> \<a>\<n>\<d> _\<close>
+                     if \<open>PLPR_Env.boolean_flag \<^const_name>\<open>ToA_flag_deep\<close> true o fst\<close>]:
+  " x \<Ztypecolon> T \<i>\<m>\<p>\<l>\<i>\<e>\<s> x' \<Ztypecolon> T' \<a>\<n>\<d> P
+\<Longrightarrow> R\<heavy_comma> x \<Ztypecolon> Var var T \<i>\<m>\<p>\<l>\<i>\<e>\<s> R\<heavy_comma> \<blangle> x' \<Ztypecolon> Var var T' \<brangle> \<a>\<n>\<d> P "
+  unfolding Action_Tag_def FOCUS_TAG_def
+  by (simp add: Var_transformation implies_left_prod)
+
+lemma [\<phi>reason 1310]:
+    \<comment> \<open>attempts the immediate cell\<close>
+  " FAIL TEXT(\<open>Variable\<close> var \<open>has not been initialized.\<close>)
+\<Longrightarrow> R \<heavy_comma> \<u>\<n>\<i>\<n>\<i>\<t>\<e>\<d> \<v>\<a>\<r>[var] \<i>\<m>\<p>\<l>\<i>\<e>\<s> R \<heavy_comma> \<blangle> x' \<Ztypecolon> \<v>\<a>\<r>[var] T' \<brangle> \<a>\<n>\<d> P"
+  unfolding Action_Tag_def by blast
+
+lemma [\<phi>reason 1280]:
+  \<open> R \<i>\<m>\<p>\<l>\<i>\<e>\<s> R' \<heavy_comma> \<blangle> x \<Ztypecolon> Var var T \<brangle> \<a>\<n>\<d> P
+\<Longrightarrow> R \<heavy_comma> H \<i>\<m>\<p>\<l>\<i>\<e>\<s> R' \<heavy_comma> H \<heavy_comma> \<blangle> x \<Ztypecolon> Var var T \<brangle> \<a>\<n>\<d> P\<close>
+  using ToSA_skip .
+
+lemma Var_simp_cong:
+  \<open> (x \<Ztypecolon> T) = (x' \<Ztypecolon> T')
+\<Longrightarrow> (x \<Ztypecolon> \<v>\<a>\<r>[v] T) = (x' \<Ztypecolon> \<v>\<a>\<r>[v] T')\<close>
+  unfolding set_eq_iff by (simp add: \<phi>expns)
+
+simproc_setup Var_simp_cong ("x \<Ztypecolon> Var v T") = \<open>
+  K (Phi_SimpCong.simproc @{thm Var_simp_cong[folded atomize_eq]})
+\<close>
+
+
+lemma [\<phi>reason 1200 for \<open>PROP Branch_Convergence_Type_Pattern (Var ?v ?T) ?X\<close>]:
+  \<open> PROP Branch_Convergence_Type_Pattern (Var v T) (Var v T')\<close>
+  unfolding Branch_Convergence_Type_Pattern_def ..
+
+
+lemma [\<phi>reason 2000]:
+  \<open> x \<Ztypecolon> T \<i>\<m>\<p>\<l>\<i>\<e>\<s> y \<Ztypecolon> U \<a>\<n>\<d> P @action to Z
+\<Longrightarrow> x \<Ztypecolon> Var v T \<i>\<m>\<p>\<l>\<i>\<e>\<s> y \<Ztypecolon> Var v U \<a>\<n>\<d> P @action to Z \<close>
+  unfolding Action_Tag_def
+  using Var_transformation .
+
+lemma [\<phi>reason 2100]:
+  \<open> x \<Ztypecolon> T \<i>\<m>\<p>\<l>\<i>\<e>\<s> y \<Ztypecolon> U \<a>\<n>\<d> P @action to Z
+\<Longrightarrow> x \<Ztypecolon> Var v T \<i>\<m>\<p>\<l>\<i>\<e>\<s> y \<Ztypecolon> Var v U \<a>\<n>\<d> P @action to (Var v Z) \<close>
+  unfolding Action_Tag_def
+  using Var_transformation .
+
+lemma [\<phi>reason 2000]:
+  \<open> x \<Ztypecolon> T \<i>\<m>\<p>\<l>\<i>\<e>\<s> y \<Ztypecolon> U \<a>\<n>\<d> P @action as Z
+\<Longrightarrow> x \<Ztypecolon> Var v T \<i>\<m>\<p>\<l>\<i>\<e>\<s> y \<Ztypecolon> Var v U \<a>\<n>\<d> P @action as Z \<close>
+  unfolding Action_Tag_def
+  using Var_transformation .
+
+lemma [\<phi>reason 2100]:
+  \<open> x \<Ztypecolon> T \<i>\<m>\<p>\<l>\<i>\<e>\<s> y \<Ztypecolon> U \<a>\<n>\<d> P @action as (z \<Ztypecolon> Z)
+\<Longrightarrow> x \<Ztypecolon> Var v T \<i>\<m>\<p>\<l>\<i>\<e>\<s> y \<Ztypecolon> Var v U \<a>\<n>\<d> P @action as (z \<Ztypecolon> Var v Z) \<close>
+  unfolding Action_Tag_def
+  using Var_transformation .
+
+
+subsubsection \<open>Application Methods for Subtyping\<close>
+
+lemma [\<phi>reason 2000 for \<open>
+  PROP \<phi>Application (Trueprop (?x \<Ztypecolon> ?T \<i>\<m>\<p>\<l>\<i>\<e>\<s> ?y \<Ztypecolon> ?U \<a>\<n>\<d> ?P))
+          (Trueprop (\<c>\<u>\<r>\<r>\<e>\<n>\<t> ?blk [?RR] \<r>\<e>\<s>\<u>\<l>\<t>\<s> \<i>\<n> ?R\<heavy_comma> ?x \<Ztypecolon> Var ?var ?T)) ?Result
+\<close> except \<open>
+  PROP \<phi>Application (Trueprop (?x \<Ztypecolon> Var ?var ?T \<i>\<m>\<p>\<l>\<i>\<e>\<s> ?y \<Ztypecolon> ?U \<a>\<n>\<d> ?P))
+          (Trueprop (\<c>\<u>\<r>\<r>\<e>\<n>\<t> ?blk [?RR] \<r>\<e>\<s>\<u>\<l>\<t>\<s> \<i>\<n> ?R)) ?Result
+\<close>]:
+  \<open> PROP \<phi>Application (Trueprop (x \<Ztypecolon> T \<i>\<m>\<p>\<l>\<i>\<e>\<s> y \<Ztypecolon> U \<a>\<n>\<d> P))
+      (Trueprop (\<c>\<u>\<r>\<r>\<e>\<n>\<t> blk [RR] \<r>\<e>\<s>\<u>\<l>\<t>\<s> \<i>\<n> R\<heavy_comma> x \<Ztypecolon> Var var T))
+      (Trueprop ((\<c>\<u>\<r>\<r>\<e>\<n>\<t> blk [RR] \<r>\<e>\<s>\<u>\<l>\<t>\<s> \<i>\<n> R\<heavy_comma> y \<Ztypecolon> Var var U) \<and> P))\<close>
+  unfolding \<phi>Application_def
+  by (meson Var_transformation \<phi>apply_implication implies_left_prod)
+
+
+lemma [\<phi>reason 2000 for \<open>
+  PROP \<phi>Application (Trueprop (?x' \<Ztypecolon> ?T' \<i>\<m>\<p>\<l>\<i>\<e>\<s> ?y \<Ztypecolon> ?U \<a>\<n>\<d> ?P))
+      (Trueprop (\<c>\<u>\<r>\<r>\<e>\<n>\<t> ?blk [?RR] \<r>\<e>\<s>\<u>\<l>\<t>\<s> \<i>\<n> ?R\<heavy_comma> ?x \<Ztypecolon> Var ?var ?T)) ?Result
+\<close> except \<open>
+  PROP \<phi>Application (Trueprop (?x \<Ztypecolon> Var ?var ?T \<i>\<m>\<p>\<l>\<i>\<e>\<s> ?y \<Ztypecolon> ?U \<a>\<n>\<d> ?P))
+          (Trueprop (\<c>\<u>\<r>\<r>\<e>\<n>\<t> ?blk [?RR] \<r>\<e>\<s>\<u>\<l>\<t>\<s> \<i>\<n> ?R)) ?Result
+\<close>]:
+  \<open> SUBGOAL TOP_GOAL G
+\<Longrightarrow> x \<Ztypecolon> T \<i>\<m>\<p>\<l>\<i>\<e>\<s> x' \<Ztypecolon> T' \<a>\<n>\<d> Any
+\<Longrightarrow> SOLVE_SUBGOAL G
+\<Longrightarrow> \<o>\<b>\<l>\<i>\<g>\<a>\<t>\<i>\<o>\<n> True
+\<Longrightarrow> PROP \<phi>Application (Trueprop (x' \<Ztypecolon> T' \<i>\<m>\<p>\<l>\<i>\<e>\<s> y \<Ztypecolon> U \<a>\<n>\<d> P))
+      (Trueprop (\<c>\<u>\<r>\<r>\<e>\<n>\<t> blk [RR] \<r>\<e>\<s>\<u>\<l>\<t>\<s> \<i>\<n> R\<heavy_comma> x \<Ztypecolon> Var var T))
+      (Trueprop ((\<c>\<u>\<r>\<r>\<e>\<n>\<t> blk [RR] \<r>\<e>\<s>\<u>\<l>\<t>\<s> \<i>\<n> R\<heavy_comma> y \<Ztypecolon> Var var U) \<and> P))\<close>
+  unfolding \<phi>Application_def
+  by (meson Var_transformation \<phi>apply_implication implies_left_prod)
+
+
+section \<open>Instructions\<close>
+
+subsection \<open>Preliminary - Reasoning Process\<close>
+
+subsubsection \<open>Infer Semantic Type of Variable\<close>
+
+consts infer_var_type :: \<open>action\<close>
+
+lemma [\<phi>reason 1000]:
+  \<open> varname.type var \<equiv> TY'
+\<Longrightarrow> pred_option ((=) TY) TY' @action infer_var_type
+\<Longrightarrow> pred_option ((=) TY) (varname.type var) @action infer_var_type\<close>
+  \<comment> \<open>TY is the output. The rule invokes evaluation of the \<open>varname.type var\<close>.\<close>
+  by simp
+
+lemma [\<phi>reason 1000]:
+  \<open>pred_option ((=) TY) None @action infer_var_type\<close>
+  \<comment> \<open>the output TY can be anything freely\<close>
+  by simp
+
+lemma [\<phi>reason 1000 for \<open>pred_option ((=) ?TY') (Some ?TY) @action infer_var_type\<close>]:
+  \<open>pred_option ((=) TY) (Some TY) @action infer_var_type\<close>
+  \<comment> \<open>the output TY equals to that TY in \<open>Some TY\<close> exactly.\<close>
+  by simp
+
+(*
+lemma
+  \<open>pred_option (\<lambda>TY'. TY = TY') None\<close>
+  \<open>pred_option (\<lambda>TY'. TY = TY') (Some TY)\<close>
+  by simp+ *)
+
+subsection \<open>Variable Operations\<close>
+
+declare [[\<phi>trace_reasoning = 2]]
+
+proc op_get_var:
+  input  \<open>x \<Ztypecolon> \<v>\<a>\<r>[var] T\<close>
+  requires [unfolded \<phi>SemType_def, useful]: \<open>\<phi>SemType (x \<Ztypecolon> T) TY\<close>
+  output \<open>x \<Ztypecolon> \<v>\<a>\<r>[var] T\<heavy_comma> x \<Ztypecolon> \<v>\<a>\<l> T\<close>
+\<medium_left_bracket>
+  (* to Identity
+  unfold Inited_Var_identity_eq *)
+  FIC.Var.getter_rule
+;;semantic_assert \<open>nosep.dest (\<phi>arg.dest \<v>0) \<in> Some ` Well_Type TY\<close>
+  semantic_return \<open>the (nosep.dest (\<phi>arg.dest \<v>0)) \<in> (x \<Ztypecolon> T)\<close>
+  fold Inited_Var_identity_eq
+\<medium_right_bracket> .
+
+proc op_set_var:
+  input  \<open>x \<Ztypecolon> Var var T\<heavy_comma> y \<Ztypecolon> \<v>\<a>\<l> U\<close>
+  requires [unfolded Action_Tag_def, useful]:
+      \<open>pred_option (\<lambda>TY'. TY = TY') (varname.type var) @action infer_var_type\<close>
+  requires \<open>\<phi>SemType (y \<Ztypecolon> U) TY\<close>
+  output \<open>y \<Ztypecolon> \<v>\<a>\<r>[var] U\<close>
+\<medium_left_bracket>
+  $y semantic_local_value TY
+  \<open>var\<close> to Identity
+  unfold Raw_Var_identity_eq
+  FIC.Var.setter_rule[where u=\<open>Some (nosep (Some (\<phi>arg.dest \<a>\<r>\<g>1)))\<close>]
+  fold Inited_Var_identity_eq
+\<medium_right_bracket> .
+
+proc op_free_var:
+  input  \<open>x \<Ztypecolon> Var var T\<close>
+  output \<open>Void\<close>
+\<medium_left_bracket>
+  to Identity
+  unfold Raw_Var_identity_eq
+  FIC.Var.setter_rule[where u=\<open>None\<close>]
+\<medium_right_bracket> .
+
+proc op_var_scope:
+  requires BLK: \<open>\<And>var. varname.type var \<equiv> TY
+                  \<Longrightarrow> \<p>\<r>\<o>\<c> F var \<lbrace> X\<heavy_comma> \<u>\<n>\<i>\<n>\<i>\<t>\<e>\<d> \<v>\<a>\<r>[var] \<longmapsto> \<lambda>ret. Y ret\<heavy_comma> () \<Ztypecolon> Var var \<phi>Any \<rbrace>
+                      \<t>\<h>\<r>\<o>\<w>\<s> (\<lambda>v. E v \<heavy_comma> () \<Ztypecolon> Var var \<phi>Any) \<close>
+  input  \<open>X\<close>
+  output \<open>Y\<close>
+  throws  E
+  \<medium_left_bracket>
+    FIC.Var.allocate_rule[where P=\<open>(\<lambda>v. varname.type v = TY)\<close> and u=\<open>Some (nosep None)\<close>] \<exists>v
+    as \<open>\<u>\<n>\<i>\<n>\<i>\<t>\<e>\<d> \<v>\<a>\<r>[v]\<close>
+thm UnInited_Var_identity_eq
+    
+    thm FIC.Var.allocate_rule[where P=\<open>(\<lambda>v. varname.type v = TY)\<close> and u=\<open>Some (nosep None)\<close>]
+
+definition op_var_scope' :: "TY option \<Rightarrow> (varname \<Rightarrow> 'ret proc) \<Rightarrow> 'ret proc"
+  where "op_var_scope' TY F =
+    RES.Var.\<phi>R_allocate_res_entry (\<lambda>v. varname.type v = TY) (Some (nosep None)) F"
+
+
+;; op_var_scope'[where TY=TY]
+    try''
+    \<medium_left_bracket> premises [\<phi>reason]  
+      BLK to Identity op_free_var \<medium_right_bracket>
+    \<medium_left_bracket> to Identity
+      op_free_var
+      throw \<medium_right_bracket>
+  \<medium_right_bracket>.
+
+lemma op_var_scope':
+   \<open>(\<And>var. varname.type var \<equiv> TY \<Longrightarrow> \<p>\<r>\<o>\<c> F var \<lbrace> X\<heavy_comma> \<u>\<n>\<i>\<n>\<i>\<t>\<e>\<d> \<v>\<a>\<r>[var] \<longmapsto> Y \<rbrace> \<t>\<h>\<r>\<o>\<w>\<s> E  )
+\<Longrightarrow> \<p>\<r>\<o>\<c> op_var_scope' TY F \<lbrace> X \<longmapsto> Y \<rbrace> \<t>\<h>\<r>\<o>\<w>\<s> E \<close>
+  unfolding op_var_scope'_def UnInited_Var_identity_eq
+  thm FIC.Var.\<phi>R_allocate_res_entry
+  apply (rule FIC.Var.\<phi>R_allocate_res_entry; simp)
+  using finite_map_freshness' infinite_varname by blast
+
+definition op_free_var :: "varname \<Rightarrow> unit proc"
+  where "op_free_var vname = RES.Var.\<phi>R_set_res (\<lambda>f. f(vname := None))"
+
+definition op_var_scope' :: "TY option \<Rightarrow> (varname \<Rightarrow> 'ret proc) \<Rightarrow> 'ret proc"
+  where "op_var_scope' TY F =
+    RES.Var.\<phi>R_allocate_res_entry (\<lambda>v. varname.type v = TY) (Some (nosep None)) F"
+
+lemma \<phi>M_get_var[intro!]:
+  \<open> v \<in> Well_Type TY
+\<Longrightarrow> \<p>\<r>\<o>\<c> F v \<lbrace> v \<Ztypecolon> \<v>\<a>\<r>[var] Identity \<longmapsto> Y \<rbrace>
+\<Longrightarrow> \<p>\<r>\<o>\<c> \<phi>M_get_var var TY F \<lbrace> v \<Ztypecolon> \<v>\<a>\<r>[var] Identity \<longmapsto> Y \<rbrace>\<close>
+  unfolding \<phi>M_get_var_def Inited_Var_identity_eq
+  by (rule FIC.Var.\<phi>R_get_res_entry; simp)
+
+lemma \<phi>M_set_var[intro!]:
+  \<open>\<p>\<r>\<o>\<c> RES.Var.\<phi>R_set_res (\<lambda>f. f(vname \<mapsto> nosep (Some u)))
+      \<lbrace> v \<Ztypecolon> Var vname Identity \<longmapsto> \<lambda>_. u \<Ztypecolon> \<v>\<a>\<r>[vname] Identity \<rbrace>\<close>
+  unfolding Inited_Var_identity_eq
+  unfolding Raw_Var_identity_eq
+  thm FIC.Var.\<phi>R_set_res
+  by (rule FIC.Var.\<phi>R_set_res[where P=\<open>\<lambda>_. True\<close>]; simp)
+
+lemma op_get_var''_\<phi>app:
+   \<open>\<p>\<r>\<e>\<m>\<i>\<s>\<e> v \<in> Well_Type TY
+\<Longrightarrow> \<p>\<r>\<o>\<c> op_get_var var TY \<lbrace> v \<Ztypecolon> \<v>\<a>\<r>[var] Identity \<longmapsto> v \<Ztypecolon> \<v>\<a>\<r>[var] Identity \<heavy_comma> \<v>\<a>\<l> v \<Ztypecolon> Identity \<rbrace>\<close>
+  unfolding op_get_var_def Premise_def
+  by (rule; rule; simp add: \<phi>expns)
+
+declare \<phi>MapAt_def[\<phi>expns del] (*HOT FIX! TESTING!*)
+
+lemma op_set_var''_\<phi>app:
+   \<open>\<p>\<r>\<e>\<m>\<i>\<s>\<e> pred_option (\<lambda>TY'. TY = TY') (varname.type var)
+\<Longrightarrow> \<p>\<r>\<e>\<m>\<i>\<s>\<e> u \<in> Well_Type TY
+\<Longrightarrow> \<p>\<r>\<o>\<c> op_set_var var TY raw \<lbrace> v \<Ztypecolon> Var var Identity\<heavy_comma> u \<Ztypecolon> \<v>\<a>\<l>[raw] Identity \<longmapsto> u \<Ztypecolon> \<v>\<a>\<r>[var] Identity \<rbrace>\<close>
+  unfolding op_set_var_def Premise_def
+  by (cases raw; simp; rule; simp add: \<phi>expns; rule)
+
+lemma finite_map_freshness':
+  \<open>finite (dom f) \<Longrightarrow> infinite P \<Longrightarrow> \<exists>x. f x = None \<and> x \<in> P\<close>
+  by (meson domIff finite_subset subsetI)
+
+lemma op_var_scope':
+   \<open>(\<And>var. varname.type var \<equiv> TY \<Longrightarrow> \<p>\<r>\<o>\<c> F var \<lbrace> X\<heavy_comma> \<u>\<n>\<i>\<n>\<i>\<t>\<e>\<d> \<v>\<a>\<r>[var] \<longmapsto> Y \<rbrace> \<t>\<h>\<r>\<o>\<w>\<s> E  )
+\<Longrightarrow> \<p>\<r>\<o>\<c> op_var_scope' TY F \<lbrace> X \<longmapsto> Y \<rbrace> \<t>\<h>\<r>\<o>\<w>\<s> E \<close>
+  unfolding op_var_scope'_def UnInited_Var_identity_eq
+  thm FIC.Var.\<phi>R_allocate_res_entry
+  apply (rule FIC.Var.\<phi>R_allocate_res_entry; simp)
+  using finite_map_freshness' infinite_varname by blast
+
+lemma op_free_var:
+   \<open>\<p>\<r>\<o>\<c> op_free_var vname \<lbrace> v \<Ztypecolon> Var vname Identity \<longmapsto> \<lambda>_. Void \<rbrace>\<close>
+  unfolding op_free_var_def Raw_Var_identity_eq
+  by (rule FIC.Var.\<phi>R_dispose_res[where P=\<open>\<lambda>_. True\<close>]; simp)
+
+
+
+section \<open>IDE-CP Operations\<close>
+
+
+
+
+
+
+ 
+subsection \<open>Rules of Variable Operations\<close>
+  
+subsubsection \<open>Get\<close> 
+
+proc [\<phi>reason 1200]:
+  input \<open>X\<close>
+  requires Find: \<open>X \<i>\<m>\<p>\<l>\<i>\<e>\<s> x \<Ztypecolon> \<v>\<a>\<r>[var] T \<r>\<e>\<m>\<a>\<i>\<n>\<s> Y \<a>\<n>\<d> Any\<close>
+      and  \<open>\<phi>SemType (x \<Ztypecolon> T) TY\<close>
+  output \<open>\<v>\<a>\<l> x <val-of> var \<Ztypecolon> T \<r>\<e>\<m>\<a>\<i>\<n>\<s> Y\<heavy_comma> x \<Ztypecolon> \<v>\<a>\<r>[var] T\<close>
+  @action synthesis
+\<medium_left_bracket>
+  Find
+  op_get_var
+\<medium_right_bracket>.
+
+
+
+subsubsection \<open>Set\<close>
+
+lemma op_set_var__synthesis [\<phi>reason 1200 for
+  \<open>\<p>\<r>\<o>\<c> ?f \<lbrace> ?R \<longmapsto> \<lambda>ret. ?R'\<heavy_comma> \<blangle> (?y <set-to> ?var) \<Ztypecolon> ?U ret \<brangle> \<rbrace> \<t>\<h>\<r>\<o>\<w>\<s> ?E  @action synthesis\<close>
+]:
+assumes G: \<open>\<p>\<r>\<o>\<c> g \<lbrace> X \<longmapsto> X1\<heavy_comma> \<blangle> \<v>\<a>\<l> y \<Ztypecolon> U \<brangle> \<rbrace> \<t>\<h>\<r>\<o>\<w>\<s> E @action synthesis \<close>
+  and P: \<open>pred_option (\<lambda>TY'. TY = TY') (varname.type var) @action infer_var_type\<close>
+  and S[unfolded Action_Tag_def]:
+         \<open>X1 \<i>\<m>\<p>\<l>\<i>\<e>\<s> Y\<heavy_comma> x \<Ztypecolon> Var var T \<a>\<n>\<d> Any @action ToSA\<close>
+  and [\<phi>reason]: \<open>\<phi>SemType (y \<Ztypecolon> U) TY\<close>
+shows \<open>\<p>\<r>\<o>\<c> (g \<bind> (\<lambda>\<v>0. op_set_var var TY \<v>0 \<ggreater> (op_get_var var TY)))
+            \<lbrace> X \<longmapsto> Y\<heavy_comma> y \<Ztypecolon> \<v>\<a>\<r>[var] U \<heavy_comma> \<blangle> \<v>\<a>\<l> (y <set-to> var) \<Ztypecolon> U \<brangle> \<rbrace>
+       \<t>\<h>\<r>\<o>\<w>\<s> E  @action synthesis\<close>
+  \<medium_left_bracket> G S op_set_var P op_get_var \<medium_right_bracket>.
+
+
+subsubsection \<open>Declare New Variables\<close>
+ 
+proc op_var_scope:
+  assumes BLK: \<open>\<And>var. varname.type var \<equiv> TY
+                  \<Longrightarrow> \<p>\<r>\<o>\<c> F var \<lbrace> X\<heavy_comma> \<u>\<n>\<i>\<n>\<i>\<t>\<e>\<d> \<v>\<a>\<r>[var] \<longmapsto> \<lambda>ret. Y ret\<heavy_comma> () \<Ztypecolon> Var var \<phi>Any
+                      \<rbrace> \<t>\<h>\<r>\<o>\<w>\<s> (\<lambda>v. E v \<heavy_comma> () \<Ztypecolon> Var var \<phi>Any) \<close>
+  input  \<open>X\<close>
+  output \<open>Y\<close>
+  throws  E
+  \<medium_left_bracket> op_var_scope'[where TY=TY]
+    try''
+    \<medium_left_bracket> premises [\<phi>reason]  
+      BLK to Identity op_free_var \<medium_right_bracket>
+    \<medium_left_bracket> to Identity
+      op_free_var
+      throw \<medium_right_bracket>
+  \<medium_right_bracket>.
+
+subsection \<open>Implementing IDE-CP Generic Variable Access\<close>
+
+lemma "__set_var_rule__":
+  \<open> \<p>\<r>\<o>\<c> g \<lbrace> R\<heavy_comma> y \<Ztypecolon> \<v>\<a>\<r>[var] U\<heavy_comma> \<blangle> X \<brangle> \<longmapsto> Z \<rbrace> \<t>\<h>\<r>\<o>\<w>\<s> E
+\<Longrightarrow> pred_option (\<lambda>TY'. TY = TY') (varname.type var) @action infer_var_type
+\<Longrightarrow> \<phi>SemType (y \<Ztypecolon> U) TY
+\<Longrightarrow> \<p>\<r>\<o>\<c> (op_set_var var TY raw \<ggreater> g) \<lbrace> R\<heavy_comma> \<blangle> x \<Ztypecolon> Var var T \<heavy_comma> y \<Ztypecolon> \<v>\<a>\<l>[raw] U\<heavy_comma> X \<brangle> \<longmapsto> Z \<rbrace> \<t>\<h>\<r>\<o>\<w>\<s> E \<close>
+  \<medium_left_bracket> premises G and P and [\<phi>reason]
+    op_set_var P G
+  \<medium_right_bracket>.
+
+lemma "__new_var_rule__":
+  \<open> (\<And>var. varname.type var \<equiv> TY
+              \<Longrightarrow> \<p>\<r>\<o>\<c> g var \<lbrace> R\<heavy_comma> \<u>\<n>\<i>\<n>\<i>\<t>\<e>\<d> \<v>\<a>\<r>[var]\<heavy_comma> \<blangle> X \<brangle> \<longmapsto> \<lambda>ret. Z ret \<heavy_comma> () \<Ztypecolon> Var var \<phi>Any
+                             \<rbrace> \<t>\<h>\<r>\<o>\<w>\<s> (\<lambda>e. E e\<heavy_comma> () \<Ztypecolon> Var var \<phi>Any))
+\<Longrightarrow> \<p>\<r>\<o>\<c> op_var_scope TYPE('a) TY g \<lbrace> R\<heavy_comma> \<blangle> X \<brangle> \<longmapsto> Z \<rbrace> \<t>\<h>\<r>\<o>\<w>\<s> E \<close>
+  \<medium_left_bracket> premises G
+    op_var_scope[where TY=\<open>TY\<close>] \<medium_left_bracket> premises [\<phi>reason for \<open>varname.type var \<equiv> _\<close>] G \<medium_right_bracket>
+  \<medium_right_bracket> .
+
+
+lemma "__set_new_var_rule__":
+  \<open> (\<And>var. varname.type var \<equiv> Some TY
+              \<Longrightarrow> \<p>\<r>\<o>\<c> g var \<lbrace> R\<heavy_comma> y \<Ztypecolon> \<v>\<a>\<r>[var] U\<heavy_comma> \<blangle> X \<brangle> \<longmapsto> \<lambda>ret. Z ret \<heavy_comma> () \<Ztypecolon> Var var \<phi>Any
+                             \<rbrace> \<t>\<h>\<r>\<o>\<w>\<s> (\<lambda>e. E e\<heavy_comma> () \<Ztypecolon> Var var \<phi>Any ))
+\<Longrightarrow> \<phi>SemType (y \<Ztypecolon> U) TY
+\<Longrightarrow> \<p>\<r>\<o>\<c> op_var_scope TYPE('a) (Some TY) (\<lambda>var. op_set_var var TY raw \<ggreater> g var)
+     \<lbrace> R\<heavy_comma> \<blangle> y \<Ztypecolon> \<v>\<a>\<l>[raw] U\<heavy_comma> X \<brangle> \<longmapsto> Z \<rbrace> \<t>\<h>\<r>\<o>\<w>\<s> E \<close>
+  \<medium_left_bracket> premises G and [\<phi>reason]
+    op_var_scope[where TY=\<open>Some TY\<close>] \<medium_left_bracket> premises [\<phi>reason for \<open>varname.type var \<equiv> _\<close>]
+      op_set_var G
+    \<medium_right_bracket>
+  \<medium_right_bracket>.
+
+lemma "__set_new_var_noty_rule__":
+  \<open> (\<And>var. varname.type var \<equiv> None
+              \<Longrightarrow> \<p>\<r>\<o>\<c> g var \<lbrace> R\<heavy_comma> y \<Ztypecolon> \<v>\<a>\<r>[var] U\<heavy_comma> \<blangle> X \<brangle> \<longmapsto> \<lambda>ret. Z ret \<heavy_comma> () \<Ztypecolon> Var var \<phi>Any
+                             \<rbrace> \<t>\<h>\<r>\<o>\<w>\<s> (\<lambda>e. E e\<heavy_comma> () \<Ztypecolon> Var var \<phi>Any))
+\<Longrightarrow> \<phi>SemType (y \<Ztypecolon> U) TY
+\<Longrightarrow> \<p>\<r>\<o>\<c> op_var_scope TYPE('a) None (\<lambda>var. op_set_var var TY raw \<ggreater> g var)
+     \<lbrace> R\<heavy_comma> \<blangle> y \<Ztypecolon> \<v>\<a>\<l>[raw] U\<heavy_comma> X \<brangle> \<longmapsto> Z \<rbrace> \<t>\<h>\<r>\<o>\<w>\<s> E \<close>
+  \<medium_left_bracket> premises G and [\<phi>reason]
+    op_var_scope[where TY=None] \<medium_left_bracket> premises [\<phi>reason for \<open>varname.type var \<equiv> _\<close>]
+      op_set_var G
+    \<medium_right_bracket>
+  \<medium_right_bracket>.
+
+ML_file "library/variable.ML"
+
+
+setup \<open>Context.theory_map (Generic_Variable_Access.Process_of_Argument.put NONE)\<close>
+
+end
+
+
