Phi_System/Calculus_of_Programming.thy
@@ -388,7 +388,7 @@ lemma introduce_Ex_ToA_subj:
 paragraph \<open>Return\<close>
 
 
-lemma \<phi>M_Success[intro!]:
+lemma \<phi>M_Success[intro!]: (*depreciated?*)
   \<open> v \<in> (y \<Ztypecolon> T)
 \<Longrightarrow> \<p>\<r>\<o>\<c> Return (\<phi>arg v) \<lbrace> X \<longmapsto> \<lambda>u. X\<heavy_comma> y \<Ztypecolon> Val u T \<rbrace> \<t>\<h>\<r>\<o>\<w>\<s> Any \<close>
   unfolding \<phi>Procedure_def det_lift_def Return_def
@@ -399,6 +399,5 @@ declare \<phi>M_Success[where X=1, simplified, intro!]
 lemma \<phi>M_Success'[intro!]:
   \<open> \<p>\<r>\<o>\<c> Return vs \<lbrace> X vs \<longmapsto> X \<rbrace> \<t>\<h>\<r>\<o>\<w>\<s> Any \<close>
   unfolding Return_def \<phi>Procedure_def det_lift_def by (clarsimp simp add: \<phi>expns)
-
 
 end
