Phi_System/PhiSem_Formalization_Tools'.thy
@@ -431,9 +431,9 @@ lemma [\<phi>reason 1200]:
 
 
 lemma [\<phi>reason 1200]:
-  \<open> \<r>Clean (x \<Ztypecolon> T)
-\<Longrightarrow> \<r>Clean (x \<Ztypecolon> \<phi> T) \<close>
-  unfolding \<r>Clean_def Imply_def apply (simp add: \<phi>expns)
+  \<open> Is_Stateless (x \<Ztypecolon> T)
+\<Longrightarrow> Is_Stateless (x \<Ztypecolon> \<phi> T) \<close>
+  unfolding Is_Stateless_def Imply_def apply (simp add: \<phi>expns)
   using mk_homo_one by blast
 
 lemma [\<phi>reason 1200 for \<open>If _ (_ \<Ztypecolon> \<phi> _) (_ \<Ztypecolon> \<phi> _) \<i>\<m>\<p>\<l>\<i>\<e>\<s> _ @action branch_convergence\<close>]:
@@ -1834,7 +1834,7 @@ definition op_set_element :: "nat list \<Rightarrow> TY \<Rightarrow> (VAL,'RES_
   ))"
 
 lemma (in \<phi>empty) op_get_element:
-  \<open> \<g>\<u>\<a>\<r>\<d> valid_index TY idx
+  \<open> \<c>\<o>\<n>\<d>\<i>\<t>\<i>\<o>\<n> valid_index TY idx
 \<Longrightarrow> \<phi>SemType (x \<Ztypecolon> X) TY
 \<Longrightarrow> \<phi>Index_getter idx X Y f
 \<Longrightarrow> \<p>\<r>\<o>\<c> op_get_element idx TY \<lbrace> VAL x \<Ztypecolon> X \<longmapsto> VAL f x \<Ztypecolon> Y \<rbrace> \<close>
@@ -1843,7 +1843,7 @@ lemma (in \<phi>empty) op_get_element:
   by \<phi>reason
 
 lemma (in \<phi>empty) op_set_element:
-  \<open> \<g>\<u>\<a>\<r>\<d> valid_index TY idx
+  \<open> \<c>\<o>\<n>\<d>\<i>\<t>\<i>\<o>\<n> valid_index TY idx
 \<Longrightarrow> \<phi>Index_mapper idx X Y f
 \<Longrightarrow> \<phi>SemType (x \<Ztypecolon> X) TY
 \<Longrightarrow> \<phi>SemType (y \<Ztypecolon> Y) (index_type idx TY)
