Phi_System/PhiSem_Formalization_Tools.thy
@@ -377,11 +377,24 @@ lemma [THEN SE_clean_waste', \<phi>reason 1211]:
   by (blast intro: \<phi>_Structural_Extract[unfolded Action_Tag_def]
                    Structural_Extract_imply_P)
 
+(*
 lemma [\<phi>reason 1100]:
   \<open> Structure_Info T P
 \<Longrightarrow> Structure_Info (\<phi> T) P\<close>
   unfolding Structure_Info_def
-  by blast
+  by blast *)
+
+thm ToSA_by_structural_extraction
+    [where T=\<open>\<phi> T\<close> and U=\<open>\<phi> U\<close> for T U]
+
+declare ToSA_by_structural_extraction
+    [where T=\<open>\<phi> T\<close> and U=\<open>\<phi> U\<close> for T U,
+     \<phi>reason 1210 if \<open>PLPR_Env.boolean_flag \<^const_name>\<open>ToA_flag_deep\<close> true o fst\<close>]
+
+declare ToSA_by_structural_extraction__reverse_transformation
+    [where T=\<open>\<phi> T\<close> and U=\<open>\<phi> U\<close> and T'=\<open>\<phi> T'\<close> and U'=\<open>\<phi> U'\<close> for T T' U U',
+     \<phi>reason 1213 if \<open>PLPR_Env.boolean_flag \<^const_name>\<open>ToA_flag_deep\<close> true o fst\<close>]
+
 
 (*lemma ToSA_by_structural_extraction:
   " Structure_Info U Q
@@ -437,9 +450,9 @@ lemma [\<phi>reason 1200]:
 
 
 lemma [\<phi>reason 1200]:
-  \<open> \<r>Clean (x \<Ztypecolon> T)
-\<Longrightarrow> \<r>Clean (x \<Ztypecolon> \<phi> T) \<close>
-  unfolding \<r>Clean_def Imply_def apply (simp add: \<phi>expns)
+  \<open> Is_Stateless (x \<Ztypecolon> T)
+\<Longrightarrow> Is_Stateless (x \<Ztypecolon> \<phi> T) \<close>
+  unfolding Is_Stateless_def Imply_def apply (simp add: \<phi>expns)
   using mk_homo_one by blast
 
 lemma [\<phi>reason 1200 for \<open>If _ (_ \<Ztypecolon> \<phi> _) (_ \<Ztypecolon> \<phi> _) \<i>\<m>\<p>\<l>\<i>\<e>\<s> _ @action branch_convergence\<close>]:
@@ -1830,7 +1843,7 @@ definition op_set_element :: "nat list \<Rightarrow> TY \<Rightarrow> (VAL,'RES_
   ))"
 
 lemma (in \<phi>empty) op_get_element:
-  \<open> \<g>\<u>\<a>\<r>\<d> valid_index TY idx
+  \<open> \<c>\<o>\<n>\<d>\<i>\<t>\<i>\<o>\<n> valid_index TY idx
 \<Longrightarrow> \<phi>SemType (x \<Ztypecolon> X) TY
 \<Longrightarrow> \<phi>Index_getter idx X Y f
 \<Longrightarrow> \<p>\<r>\<o>\<c> op_get_element idx TY \<lbrace> VAL x \<Ztypecolon> X \<longmapsto> VAL f x \<Ztypecolon> Y \<rbrace> \<close>
@@ -1839,7 +1852,7 @@ lemma (in \<phi>empty) op_get_element:
   by \<phi>reason
 
 lemma (in \<phi>empty) op_set_element:
-  \<open> \<g>\<u>\<a>\<r>\<d> valid_index TY idx
+  \<open> \<c>\<o>\<n>\<d>\<i>\<t>\<i>\<o>\<n> valid_index TY idx
 \<Longrightarrow> \<phi>Index_mapper idx X Y f
 \<Longrightarrow> \<phi>SemType (x \<Ztypecolon> X) TY
 \<Longrightarrow> \<phi>SemType (y \<Ztypecolon> Y) (index_type idx TY)
