Phi_System/Phi_Preliminary.thy
@@ -46,7 +46,6 @@ subsection \<open>Helper ML\<close>
 
 ML_file \<open>library/tools/Phi_Help.ML\<close>
 ML_file \<open>library/syntax/helps.ML\<close>
-ML_file \<open>library/tools/Hook.ML\<close>
 ML_file \<open>library/system/Phi_Envir0.ML\<close>
 ML_file \<open>library/system/Phi_ID.ML\<close>
 ML_file \<open>library/tools/cache_file.ML\<close>
